Projects/AP/Alts/Alt1/Equiv.lean
@@ -1,4 +1,5 @@
 import Projects.AP.Alts.Alt1.Auxi
+import Projects.Temp
 
 namespace AP.Alt₁
 
@@ -151,7 +152,7 @@ instance : Inhabited State := ⟨state₀⟩
 @[simp]
 theorem toAltH_state₀_eq {pw} : state₀.toAltH pw = AP.initState pw 0 := by
   simp [State.toAltH, State.toAltH?, Board.toAltH?]
-  apply choose?_of (P := λ (s : Option AP.State) => s.getd = _) _ _
+  apply choose?_of_pos (P := λ (s : Option AP.State) => s.getd = _) _ _
   · use AP.initState pw 0; simp
   rintro s h ⟨h₁, h₂⟩; simp; rw [←h₂]; simp
   rw [State.hist_eq_aPos_of] <;> rw [←h₂] <;> simp
@@ -168,7 +169,7 @@ theorem initial_toAltH_state₀ {pw} : sys.Initial # state₀.toAltH pw := by
 theorem aHws_toAltH_state₀ {pw} : (state₀.toAltH pw).aHws ↔ AP.aHwsPw pw := by
   rw [aHwsPw_iff_p 0]
   simp [State.toAltH, State.toAltH?, Board.toAltH?]
-  apply choose?_of (P := λ (x : Option AP.State) => x.getd.aHws ↔ _) _ _
+  apply choose?_of_pos (P := λ (x : Option AP.State) => x.getd.aHws ↔ _) _ _
   · use AP.initState pw 0; simp
   rintro s - ⟨hs, h₂⟩
   simp at h₂ ⊢
@@ -214,6 +215,265 @@ theorem Game.act_applyDMove {s m} : (applyDMove s m).act ↔ s.act := by rfl
 theorem Game.act_playDMoveAt {pw} {g : Game pw} {h} : (playDMoveAt g h).act := by
   simpa [playDMoveAt]
 
+theorem Game.playMove_eq_of_not_act {pw} {g : Game pw} (h : ¬g.act) : g.playMove = g := by
+  simp [playMove, h]
+
+theorem Game.play_eq_of_not_act {pw} {g : Game pw} {n} (h : ¬g.act) : g.play n = g := by
+  induction n; rfl; nm n ih; rw [play_succ, ih]; exact playMove_eq_of_not_act h
+
+@[simp]
+theorem State.act_finish {s : State} : ¬s.finish.act := by
+  simp [finish]
+
+@[simp]
+theorem Game.act_finish {pw} {g : Game pw} : ¬g.finish.act := by
+  simp [finish]
+
+@[simp]
+theorem Game.playMove_finish {pw} {g : Game pw} : g.finish.playMove = g.finish := by
+  apply playMove_eq_of_not_act; simp
+
+@[simp]
+theorem Game.play_finish {pw} {g : Game pw} {n} : g.finish.play n = g.finish := by
+  apply play_eq_of_not_act; simp
+
+@[simp]
+theorem a_playDMoveAt {pw} {g : Game pw} {h} : (playDMoveAt g h).a = g.a := rfl
+
+@[simp] theorem a_initGame {pw a d s} : (initGame a d s : Game pw).a = a := rfl
+@[simp] theorem d_initGame {pw a d s} : (initGame a d s : Game pw).d = d := rfl
+
+@[simp]
+theorem State.aTurn_applyMove {s m} : (applyMove s m).aTurn = !s.aTurn := by
+  simp [applyMove, State.aTurn]
+
+@[simp]
+theorem State.aTurn_applyDMove {s m} : (applyDMove s m).aTurn = !s.aTurn := by
+  simp [applyDMove]
+
+@[simp]
+theorem aTurn_playDMoveAt {pw} {g : Game pw} {h} : (playDMoveAt g h).s.aTurn = !g.s.aTurn := by
+  simp [playDMoveAt]
+
+@[simp]
+theorem applyDMoveB_none {b} : applyDMoveB b none = b := rfl
+
+@[simp]
+theorem State.board_applyMove {s b} : (applyMove s b).board = b := rfl
+
+@[simp]
+theorem State.history_applyMove {s b} : (applyMove s b).history = s.history ++ [s.board] := rfl
+
+@[simp]
+theorem State.act_applyMove {s b} : (applyMove s b).act ↔ s.act := by rfl
+
+@[simp]
+theorem applyDMove_none {s} : applyDMove s none = s.setHist (s.history ++ [s.board]) := by
+  ext:1 <;> simp [applyDMove]
+
+@[simp]
+theorem State.aTurn_setHist {s : State} {hist} :
+(s.setHist hist).aTurn = decide (Odd hist.length) := by
+  simp [setHist]
+
+theorem State.toAltH_setHist {pw} {s : State} {hist}
+(ht : s.aTurn = decide (Odd hist.length)) :
+(s.setHist hist).toAltH pw = s.toAltH pw := by
+  simp [toAltH, toAltH?, ←ht]
+
+theorem State.wf_iff {pw} {s : State} : s.WF pw ↔ ∃ a d n g,
+(initGame a d state₀ : Game pw).play n = g ∧ (g.s = s ∨ ∃ h, (playDMoveAt g h).s = s) :=
+  ⟨λ ⟨h⟩ => h, λ h => ⟨h⟩⟩
+
+@[simp, instance]
+theorem wf_state₀ {pw} : state₀.WF pw := by
+  rw [State.wf_iff]; use default, default, 0; simp
+
+@[simp]
+theorem Game.setState_initGame {pw a d s s'} :
+(initGame a d s : Game pw).setState s' = initGame a d s' := rfl
+
+@[simp]
+theorem Game.s_finish {pw} {g : Game pw} : g.finish.s = g.s.finish := rfl
+
+@[simp]
+theorem State.aTurn_finish {s : State} : s.finish.aTurn = s.aTurn := rfl
+
+@[simp]
+theorem State.act_applyAMove {s : State} {b} : (applyAMove s b).act ↔ s.act := by rfl
+
+@[simp]
+theorem State.aTurn_applyAMove {s : State} {b} : (applyAMove s b).aTurn = !s.aTurn := by
+  simp [applyAMove]
+
+theorem Game.act_play_initGame_of_not_aTurn {pw a d n g s}
+(h₁ : s.aTurn = false) (h₂ : s.act) (h₃ : (initGame a d s : Game pw).play n = g)
+(h₄ : g.s.aTurn = false) : g.act := by
+  induction n generalizing s g
+  · simp at h₃; simpa [←h₃]
+  nm n ih
+  rw [play_succ'] at h₃
+  simp [playMove, h₂] at h₃
+  simp [playDMoveAt] at h₃
+  generalize_proofs at h₃
+  generalize h₅ : applyDMove s (d.f s h₂).m = s₁ at h₃
+  have h₆ : s₁.act; simpa [←h₅]
+  simp [playAMoveAt] at h₃
+  rw! (castMode := .all) [eq_true_of h₆, true_and] at h₃
+  split_ifs at h₃ with h₇
+  rotate_left
+  · replace h₃ := congrArg (·.s.aTurn) h₃
+    simp [←h₅, h₁, h₄] at h₃
+  simp [playAMoveAt'] at h₃
+  generalize_proofs at h₃
+  generalize hs₂ : applyAMove s₁ (a.f s₁ h₆ h₇).m = s₂ at h₃
+  have H₁ : s₂.act; simpa [←hs₂]
+  have H₂ : s₁.aTurn = true; simpa [←h₅]
+  have H₃ : s₂.aTurn = false; simpa [←hs₂]
+  grind
+
+@[simp]
+theorem Game.s_playDMoveAt_eq_iff {pw} {g₁ g₂ : Game pw} {h₁ h₂} :
+(playDMoveAt g₁ h₁).s = (playDMoveAt g₂ h₂).s ↔
+applyDMove g₁.s (g₁.d.f g₁.s h₁).m = applyDMove g₂.s (g₂.d.f g₂.s h₂).m := by rfl
+
+@[simp] theorem Game.a_finish {pw} {g : Game pw} : g.finish.a = g.a := rfl
+@[simp] theorem Game.d_finish {pw} {g : Game pw} : g.finish.d = g.d := rfl
+
+@[simp] theorem Game.a_setState {pw} {g : Game pw} {s} : (g.setState s).a = g.a := rfl
+@[simp] theorem Game.d_setState {pw} {g : Game pw} {s} : (g.setState s).d = g.d := rfl
+
+@[simp]
+theorem Game.a_playAMoveAt' {pw} {g : Game pw} {a : A pw} {h₁ h₂} :
+(playAMoveAt' a g h₁ h₂).a = g.a := rfl
+
+@[simp]
+theorem Game.d_playAMoveAt' {pw} {g : Game pw} {a : A pw} {h₁ h₂} :
+(playAMoveAt' a g h₁ h₂).d = g.d := rfl
+
+@[simp]
+theorem Game.a_playAMoveAt {pw} {g : Game pw} : (playAMoveAt g).a = g.a := by
+  simp [playAMoveAt]; split_ifs <;> simp
+
+@[simp]
+theorem Game.d_playAMoveAt {pw} {g : Game pw} : (playAMoveAt g).d = g.d := by
+  simp [playAMoveAt]; split_ifs <;> simp
+
+@[simp]
+theorem Game.a_playDMoveAt {pw} {g : Game pw} {h} : (playDMoveAt g h).a = g.a := by
+  simp [playDMoveAt]
+
+@[simp]
+theorem Game.d_playDMoveAt {pw} {g : Game pw} {h} : (playDMoveAt g h).d = g.d := by
+  simp [playDMoveAt]
+
+@[simp]
+theorem Game.a_playMove {pw} {g : Game pw} : g.playMove.a = g.a := by
+  simp [playMove]; split_ifs <;> simp
+
+@[simp]
+theorem Game.d_playMove {pw} {g : Game pw} : g.playMove.d = g.d := by
+  simp [playMove]; split_ifs <;> simp
+
+@[simp]
+theorem Game.a_play {pw} {g : Game pw} {n} : (g.play n).a = g.a := by
+  induction n; rfl; simpa [play_succ]
+
+@[simp]
+theorem Game.d_play {pw} {g : Game pw} {n} : (g.play n).d = g.d := by
+  induction n; rfl; simpa [play_succ]
+
+@[simp]
+theorem State.board_finish {s : State} : s.finish.board = s.board := rfl
+
+theorem Game.s_playAMoveAt_eq_of {pw} {g₁ g₂ : Game pw} (h₁ : g₁.s.act ↔ g₂.s.act)
+(h₂ : AHasValidMove pw g₁.s.board ↔ AHasValidMove pw g₂.s.board) : ∀ h₁ h₂ h₃ h₄,
+(playAMoveAt g₁).s = (playAMoveAt g₂).s ↔
+applyAMove g₁.s (g₁.a.f g₁.s h₁ h₂).m = applyAMove g₂.s (g₂.a.f g₂.s h₃ h₄).m := by
+  simp_all [playAMoveAt, playAMoveAt', applyAMove, act]
+
+theorem Game.playAMoveAt_eq_of_neg {pw} {g : Game pw}
+(h : ¬g.act ∨ ¬AHasValidMove pw g.s.board) : playAMoveAt g = g.finish := by
+  simp [playAMoveAt]; tauto
+
+theorem Game.s_play_initGame_d_set_eq_of_ne {pw a d s s₁ dRef n}
+(h : ∀ k < n, (initGame a d s |>.play k : Game pw).s ≠ s₁) :
+(initGame a (d.set s₁ dRef) s |>.play n).s = (initGame a d s |>.play n).s := by
+  induction n; simp
+  nm n ih
+  specialize ih # by grind
+  simp [play_succ, playMove, act]
+  rw! (castMode := .all) [ih]
+  split_ifs with h₁
+  on_goal 2 => exact ih
+  generalize hg : (initGame a d s).play n = g at *
+  generalize hg₁ : (initGame a (d.set s₁ dRef) s).play n = g₁ at *
+  have H₁ : g₁.a = g.a; simp [←hg, ←hg₁]
+  simp [playDMoveAt]
+  rw! [ih]
+  suffices h₂ : applyDMove g.s (g₁.d.f g.s h₁).m = applyDMove g.s (g.d.f g.s h₁).m
+  · rw [h₂]
+    generalize h₃ : applyDMove g.s (g.d.f g.s h₁).m = s'
+    have h₄ : s'.act; simpa [←h₃]
+    by_cases h₅ : ¬AHasValidMove pw s'.board
+    · iterate 2 rw [playAMoveAt_eq_of_neg # by tauto];; simp
+    push_neg at h₅
+    have h₆ := @s_playAMoveAt_eq_of _ (g₁.setState s') (g.setState s')
+      (by simp) (by simp) (by simpa) (by simpa) (by simpa) (by simpa)
+    rw [h₆]; clear h₆
+    simp; grind
+  congr 2; simp [←hg₁, D.set]
+  rw [if_neg]; simp [←hg]
+  rw [←hg]; apply h; omega
+
+-- theorem Game.s_play_eq_iff_of_act {pw} {g : Game pw} {n m}
+-- (h : g.play (max n m) |>.act) : (g.play n).s = (g.play m).s ↔ n = m := by
+--   sorry
+
+-- #check 0 #exit
+
+-- theorem wf_playDMoveAt {pw} {g : Game pw} {h} (hs : g.s.WF pw)
+-- (ht : g.s.aTurn = false) : (playDMoveAt g h).s.WF pw := by
+--   rw [State.wf_iff] at hs ⊢
+--   choose a d n g₁ h₁ h₂ using hs
+--   rcases h₂ with h₂ | ⟨h₂, h₃⟩
+--   ·
+--     generalize hg' : (initGame a (d.set g₁.s g.d) state₀).play n = g'
+--     refine' ⟨a, _, n, g', hg', _⟩
+--     have h₃ : g₁.s.act
+--     ·
+--       replace h₂ := congrArg (·.aTurn) h₂
+--       simp [ht] at h₂
+--       apply Game.act_play_initGame_of_not_aTurn _ _ h₁ <;> simp_all
+--     right
+--     have h₄ : g'.s = g.s
+--     ·
+--       -- rw [←h₂, ←hg', ←h₁]
+--       rw [←h₂, ←h₁, ←hg']
+--       apply Game.s_play_initGame_d_set_eq_of_ne
+--       intro k hk
+--       simp [←h₁]
+--       rw [Game.s_play_eq_iff_of_act]; omega
+--       rw [max_eq_right_of_lt hk, h₁]
+--     simp [h₄, h]
+--     simp [applyDMove, applyMove]
+--     congr 1
+--     simp [←hg']
+--     simp [D.set]
+--     grind
+--   ·
+--     sorry
+
+-- #check 0 #exit
+
+-- theorem dHws_and_dwn_lt_toAltH_playDMoveAt_dOptimal_of_dHws {pw} {g g₁ : Game pw} {h}
+-- (h₁ : g.d = (dOptimal pw).getd)
+-- (h₂ : g.s.toAltH pw |>.dHws)
+-- (ht : g.s.aTurn = false)
+-- (hg₁ : playDMoveAt g h = g₁) :
+-- (g₁.s.toAltH pw).dHws ∧ g₁.s.dwn pw < g.s.dwn pw := by
+--   sorry
+
 -- #check 0 #exit
 
 -- theorem DHws_of_alt {pw} (h : AP.dHwsPw pw) : DHws pw := by
@@ -225,7 +485,7 @@ theorem Game.act_playDMoveAt {pw} {g : Game pw} {h} : (playDMoveAt g h).act := b
 --     subst h₀
 --     simp [State.toAltH, State.toAltH?, Board.toAltH?]
 --     
---     apply choose?_of (P := λ (x : Option AP.State) => x.getd.dHws) _ _
+--     apply choose?_of_pos (P := λ (x : Option AP.State) => x.getd.dHws) _ _
 --     ·
 --       use AP.initState pw 0
 --       simp
@@ -259,6 +519,10 @@ theorem Game.act_playDMoveAt {pw} {g : Game pw} {h} : (playDMoveAt g h).act := b
 --     rw [←h₀]
 --     simp
 --   
+--   have ht : s.aTurn = false
+--   ·
+--     simp [←h₀]
+--   
 --   clear h₀ h₁
 --   
 --   use n
@@ -275,3 +539,31 @@ theorem Game.act_playDMoveAt {pw} {g : Game pw} {h} : (playDMoveAt g h).act := b
 --   simp [Game.play_succ', Game.playMove, h₃, playAMoveAt]
 --   rw! [eq_true_of Game.act_playDMoveAt]
 --   rw! (castMode := .all) [true_and]
+--   
+--   split_ifs with h₄
+--   on_goal 2 => simp
+--   
+--   generalize_proofs H₁ H₂ H₃
+--   by_contra H
+--   generalize hg₁ : playDMoveAt (initGame a d s) H₁ = g₁
+--   contrapose H; clear H
+--   rw! [hg₁] at h₄ ⊢
+--   
+--   have ht₁ : g₁.s.aTurn = true
+--   ·
+--     clear ih
+--     subst hg₁
+--     simpa
+--   
+--   obtain ⟨h₅, h₆⟩ : (g₁.s.toAltH pw).dHws ∧ g₁.s.dwn pw < s.dwn pw
+--   ·
+--     clear ih
+--     apply @dHws_and_dwn_lt_toAltH_playDMoveAt_dOptimal_of_dHws pw (initGame a d s) g₁
+--     simp [h₂]; all_goals simpa
+--   
+--   have hs₁ : sys.WF # g₁.s.toAltH pw
+--   ·
+--     clear ih
+--     simp [←hg₁]
+--   
+--   -- specialize ih _ (by omega) g₁.s h₅ rfl hs₁ (by simpa [←hg₁])
